refactor: Free simps

HepLean/PerturbationTheory/Contractions/Insert.lean
@@ -32,39 +32,41 @@ def insert (c : ContractionsNat n) (i : Fin n.succ) (j : Option (c.uncontracted)
   · simp only [Nat.succ_eq_add_one, f']
     match j with
     | none =>
-      simp [f', f]
+      simp only [Finset.le_eq_subset, Finset.mem_map, RelEmbedding.coe_toEmbedding,
+        forall_exists_index, and_imp, forall_apply_eq_imp_iff₂, f]
       intro a ha
       rw [Finset.mapEmbedding_apply]
-      simp [Finset.mapEmbedding_apply]
+      simp only [Finset.card_map]
       exact c.2.1 a ha
     | some j =>
-      simp
+      simp only [Finset.mem_insert, forall_eq_or_imp]
       apply And.intro
       · rw [@Finset.card_eq_two]
         use i
         use (i.succAbove j)
-        simp
+        simp only [ne_eq, and_true]
         exact Fin.ne_succAbove i j
       · simp only [Finset.le_eq_subset, Finset.mem_map, RelEmbedding.coe_toEmbedding,
         forall_exists_index, and_imp, forall_apply_eq_imp_iff₂, f]
         intro a ha
         rw [Finset.mapEmbedding_apply]
-        simp
+        simp only [Finset.card_map]
         exact c.2.1 a ha
   · intro a ha b hb
-    simp [f'] at ha hb
+    simp only [Nat.succ_eq_add_one, f'] at ha hb
     match j with
     | none =>
-      simp_all [f]
+      simp_all only [f, Finset.le_eq_subset, Finset.mem_map, RelEmbedding.coe_toEmbedding,
+        Nat.succ_eq_add_one]
       obtain ⟨a', ha', ha''⟩ := ha
       obtain ⟨b', hb', hb''⟩ := hb
       subst ha''
       subst hb''
-      simp
+      simp only [EmbeddingLike.apply_eq_iff_eq]
       rw [Finset.mapEmbedding_apply, Finset.mapEmbedding_apply, Finset.disjoint_map]
       exact c.2.2 a' ha' b' hb'
     | some j =>
-      simp_all
+      simp_all only [Finset.mem_insert, Nat.succ_eq_add_one]
       match ha, hb with
       | Or.inl ha, Or.inl hb =>
         rw [ha, hb]
@@ -72,15 +74,15 @@ def insert (c : ContractionsNat n) (i : Fin n.succ) (j : Option (c.uncontracted)
       | Or.inl ha, Or.inr hb =>
         apply Or.inr
         subst ha
-        simp
-        simp [f] at hb
+        simp only [Finset.disjoint_insert_left, Finset.disjoint_singleton_left]
+        simp only [Finset.le_eq_subset, Finset.mem_map, RelEmbedding.coe_toEmbedding, f] at hb
         obtain ⟨a', hb', hb''⟩ := hb
         subst hb''
         rw [Finset.mapEmbedding_apply]
         apply And.intro
-        · simp
+        · simp only [Finset.mem_map, Fin.succAboveEmb_apply, not_exists, not_and]
           exact fun x _ => Fin.succAbove_ne i x
-        · simp
+        · simp only [Finset.mem_map, Fin.succAboveEmb_apply, not_exists, not_and]
           have hj := j.2
           rw [mem_uncontracted_iff_not_contracted] at hj
           intro a ha hja
@@ -90,15 +92,16 @@ def insert (c : ContractionsNat n) (i : Fin n.succ) (j : Option (c.uncontracted)
       | Or.inr ha, Or.inl hb =>
         apply Or.inr
         subst hb
-        simp
-        simp [f] at ha
+        simp only [Finset.disjoint_insert_right, Nat.succ_eq_add_one,
+          Finset.disjoint_singleton_right]
+        simp only [Finset.le_eq_subset, Finset.mem_map, RelEmbedding.coe_toEmbedding, f] at ha
         obtain ⟨a', ha', ha''⟩ := ha
         subst ha''
         rw [Finset.mapEmbedding_apply]
         apply And.intro
-        · simp
+        · simp only [Finset.mem_map, Fin.succAboveEmb_apply, not_exists, not_and]
           exact fun x _ => Fin.succAbove_ne i x
-        · simp
+        · simp only [Finset.mem_map, Fin.succAboveEmb_apply, not_exists, not_and]
           have hj := j.2
           rw [mem_uncontracted_iff_not_contracted] at hj
           intro a ha hja
@@ -106,19 +109,20 @@ def insert (c : ContractionsNat n) (i : Fin n.succ) (j : Option (c.uncontracted)
           subst hja
           exact False.elim (hj a' ha' ha)
       | Or.inr ha, Or.inr hb =>
-        simp_all [f]
+        simp_all only [f, Finset.le_eq_subset,
+          or_true, Finset.mem_map, RelEmbedding.coe_toEmbedding]
         obtain ⟨a', ha', ha''⟩ := ha
         obtain ⟨b', hb', hb''⟩ := hb
         subst ha''
         subst hb''
-        simp
+        simp only [EmbeddingLike.apply_eq_iff_eq]
         rw [Finset.mapEmbedding_apply, Finset.mapEmbedding_apply, Finset.disjoint_map]
         exact c.2.2 a' ha' b' hb'
 
 lemma insert_of_isSome (c : ContractionsNat n) (i : Fin n.succ) (j : Option c.uncontracted)
     (hj : j.isSome) : (insert c i j).1 = Insert.insert {i, i.succAbove (j.get hj)}
     (Finset.map (Finset.mapEmbedding i.succAboveEmb).toEmbedding c.1) := by
-  simp [insert]
+  simp only [Nat.succ_eq_add_one, insert, Finset.le_eq_subset]
   rw [@Option.isSome_iff_exists] at hj
   obtain ⟨j, hj⟩ := hj
   subst hj
@@ -129,7 +133,8 @@ lemma self_mem_uncontracted_of_insert_none (c : ContractionsNat n) (i : Fin n.su
     i ∈ (insert c i none).uncontracted := by
   rw [mem_uncontracted_iff_not_contracted]
   intro p hp
-  simp [insert] at hp
+  simp only [Nat.succ_eq_add_one, insert, Finset.le_eq_subset, Finset.mem_map,
+    RelEmbedding.coe_toEmbedding] at hp
   obtain ⟨a, ha, ha'⟩ := hp
   have hc := c.2.1 a ha
   rw [@Finset.card_eq_two] at hc
@@ -137,7 +142,8 @@ lemma self_mem_uncontracted_of_insert_none (c : ContractionsNat n) (i : Fin n.su
   subst ha
   subst ha'
   rw [Finset.mapEmbedding_apply]
-  simp
+  simp only [Nat.succ_eq_add_one, Finset.map_insert, Fin.succAboveEmb_apply, Finset.map_singleton,
+    Finset.mem_insert, Finset.mem_singleton, not_or]
   apply And.intro
   · exact Fin.ne_succAbove i x
   · exact Fin.ne_succAbove i y
@@ -152,7 +158,8 @@ lemma self_not_mem_uncontracted_of_insert_some (c : ContractionsNat n) (i : Fin 
 lemma insert_succAbove_mem_uncontracted_iff (c : ContractionsNat n) (i : Fin n.succ) (j : Fin n) :
     (i.succAbove j) ∈ (insert c i none).uncontracted ↔ j ∈ c.uncontracted := by
   rw [mem_uncontracted_iff_not_contracted, mem_uncontracted_iff_not_contracted]
-  simp [insert]
+  simp only [Nat.succ_eq_add_one, insert, Finset.le_eq_subset, Finset.mem_map,
+    RelEmbedding.coe_toEmbedding, forall_exists_index, and_imp, forall_apply_eq_imp_iff₂]
   apply Iff.intro
   · intro h p hp
     have hp' := h p hp
@@ -161,8 +168,9 @@ lemma insert_succAbove_mem_uncontracted_iff (c : ContractionsNat n) (i : Fin n.s
     obtain ⟨x, y, hxy, hp⟩ := hc
     subst hp
     rw [Finset.mapEmbedding_apply] at hp'
-    simp at hp'
-    simp
+    simp only [Finset.map_insert, Fin.succAboveEmb_apply, Finset.map_singleton, Finset.mem_insert,
+      Finset.mem_singleton, not_or] at hp'
+    simp only [Finset.mem_insert, Finset.mem_singleton, not_or]
     exact And.intro (fun a => hp'.1 (congrArg i.succAbove a))
       (fun a => hp'.2 (congrArg i.succAbove a))
   · intro h p hp
@@ -171,9 +179,10 @@ lemma insert_succAbove_mem_uncontracted_iff (c : ContractionsNat n) (i : Fin n.s
     obtain ⟨x, y, hxy, hp⟩ := hc
     subst hp
     rw [Finset.mapEmbedding_apply]
-    simp
+    simp only [Finset.map_insert, Fin.succAboveEmb_apply, Finset.map_singleton, Finset.mem_insert,
+      Finset.mem_singleton, not_or]
     have hp' := h {x, y} hp
-    simp at hp'
+    simp only [Finset.mem_insert, Finset.mem_singleton, not_or] at hp'
     apply And.intro
       (fun a => hp'.1 (i.succAbove_right_injective a))
       (fun a => hp'.2 (i.succAbove_right_injective a))
@@ -185,11 +194,11 @@ lemma mem_uncontracted_insert_none_iff (c : ContractionsNat n) (i : Fin n.succ) 
   by_cases hi : k = i
   · subst hi
     simp
-  · simp [← Fin.exists_succAbove_eq_iff] at hi
+  · simp only [Nat.succ_eq_add_one, ← Fin.exists_succAbove_eq_iff] at hi
     obtain ⟨z, hk⟩ := hi
     subst hk
     have hn : ¬ i.succAbove z = i := by exact Fin.succAbove_ne i z
-    simp [hn]
+    simp only [Nat.succ_eq_add_one, insert_succAbove_mem_uncontracted_iff, hn, false_or]
     apply Iff.intro
     · intro h
       exact ⟨z, rfl, h⟩
@@ -202,7 +211,8 @@ lemma mem_uncontracted_insert_none_iff (c : ContractionsNat n) (i : Fin n.succ) 
 lemma insert_none_uncontracted (c : ContractionsNat n) (i : Fin n.succ) :
     (insert c i none).uncontracted = Insert.insert i (c.uncontracted.map i.succAboveEmb) := by
   ext a
-  simp
+  simp only [Nat.succ_eq_add_one, mem_uncontracted_insert_none_iff, Finset.mem_insert,
+    Finset.mem_map, Fin.succAboveEmb_apply]
   apply Iff.intro
   · intro a_1
     cases a_1 with
@@ -242,27 +252,33 @@ lemma mem_uncontracted_insert_some_iff (c : ContractionsNat n) (i : Fin n.succ)
     ∃ z, k = i.succAbove z ∧ z ∈ c.uncontracted ∧ z ≠ j := by
   by_cases hki : k = i
   · subst hki
-    simp
+    simp only [Nat.succ_eq_add_one, self_not_mem_uncontracted_of_insert_some, ne_eq, false_iff,
+      not_exists, not_and, Decidable.not_not]
     exact fun x hx => False.elim (Fin.ne_succAbove k x hx)
-  · simp [← Fin.exists_succAbove_eq_iff] at hki
+  · simp only [Nat.succ_eq_add_one, ← Fin.exists_succAbove_eq_iff] at hki
     obtain ⟨z, hk⟩ := hki
     subst hk
     by_cases hjz : j = z
     · subst hjz
       rw [mem_uncontracted_iff_not_contracted]
-      simp [insert]
+      simp only [Nat.succ_eq_add_one, insert, Finset.le_eq_subset, Finset.mem_insert,
+        Finset.mem_map, RelEmbedding.coe_toEmbedding, forall_eq_or_imp, Finset.mem_singleton,
+        or_true, not_true_eq_false, forall_exists_index, and_imp, forall_apply_eq_imp_iff₂,
+        false_and, ne_eq, false_iff, not_exists, not_and, Decidable.not_not]
       intro x
       rw [Function.Injective.eq_iff (Fin.succAbove_right_injective)]
       exact fun a _a => a.symm
     · apply Iff.intro
       · intro h
         use z
-        simp
+        simp only [Nat.succ_eq_add_one, ne_eq, true_and]
         refine And.intro ?_ (fun a => hjz a.symm)
         rw [mem_uncontracted_iff_not_contracted]
         intro p hp
         rw [mem_uncontracted_iff_not_contracted] at h
-        simp [insert] at h
+        simp only [Nat.succ_eq_add_one, insert, Finset.le_eq_subset, Finset.mem_insert,
+          Finset.mem_map, RelEmbedding.coe_toEmbedding, forall_eq_or_imp, Finset.mem_singleton,
+          not_or, forall_exists_index, and_imp, forall_apply_eq_imp_iff₂] at h
         have hc := h.2 p hp
         rw [Finset.mapEmbedding_apply] at hc
         exact (Finset.mem_map' (i.succAboveEmb)).mpr.mt hc
@@ -271,7 +287,9 @@ lemma mem_uncontracted_insert_some_iff (c : ContractionsNat n) (i : Fin n.succ)
         rw [Function.Injective.eq_iff (Fin.succAbove_right_injective)] at hz'1
         subst hz'1
         rw [mem_uncontracted_iff_not_contracted]
-        simp [insert]
+        simp only [Nat.succ_eq_add_one, insert, Finset.le_eq_subset, Finset.mem_insert,
+          Finset.mem_map, RelEmbedding.coe_toEmbedding, forall_eq_or_imp, Finset.mem_singleton,
+          not_or, forall_exists_index, and_imp, forall_apply_eq_imp_iff₂]
         apply And.intro
         · rw [Function.Injective.eq_iff (Fin.succAbove_right_injective)]
           exact And.intro (Fin.succAbove_ne i z) (fun a => hjz a.symm)
@@ -281,23 +299,24 @@ lemma mem_uncontracted_insert_some_iff (c : ContractionsNat n) (i : Fin n.succ)
 lemma insert_some_uncontracted (c : ContractionsNat n) (i : Fin n.succ) (j : c.uncontracted) :
     (insert c i (some j)).uncontracted = (c.uncontracted.erase j).map i.succAboveEmb := by
   ext a
-  simp
+  simp only [Nat.succ_eq_add_one, mem_uncontracted_insert_some_iff, ne_eq, Finset.map_erase,
+    Fin.succAboveEmb_apply, Finset.mem_erase, Finset.mem_map]
   apply Iff.intro
   · intro h
     obtain ⟨z, h1, h2, h3⟩ := h
     subst h1
     rw [Function.Injective.eq_iff (Fin.succAbove_right_injective)]
-    simp [h3]
+    simp only [h3, not_false_eq_true, true_and]
     use z
   · intro h
     obtain ⟨z, h1, h2⟩ := h.2
     use z
     subst h2
-    simp
+    simp only [true_and]
     obtain ⟨a, ha1, ha2⟩ := h.2
     rw [Function.Injective.eq_iff (Fin.succAbove_right_injective)] at ha2
     subst ha2
-    simp_all
+    simp_all only [true_and]
     rw [Function.Injective.eq_iff (Fin.succAbove_right_injective)] at h
     exact h.1
 
@@ -311,7 +330,7 @@ lemma insert_none_getDual?_isNone (c : ContractionsNat n) (i : Fin n.succ) :
     ((insert c i none).getDual? i).isNone := by
   have hi : i ∈ (insert c i none).uncontracted := by
     simp
-  simp [uncontracted] at hi
+  simp only [Nat.succ_eq_add_one, uncontracted, Finset.mem_filter, Finset.mem_univ, true_and] at hi
   rw [hi]
   simp
 
@@ -335,9 +354,10 @@ lemma insert_succAbove_getDual?_get (c : ContractionsNat n) (i : Fin n.succ) (j 
   have h1 : (insert c i none).getDual? (i.succAbove j) = some
       (i.succAbove ((c.getDual? j).get (by simpa using h))) := by
     rw [getDual?_eq_some_iff_mem]
-    simp [insert]
+    simp only [Nat.succ_eq_add_one, insert, Finset.le_eq_subset, Finset.mem_map,
+      RelEmbedding.coe_toEmbedding]
     use {j, ((c.getDual? j).get (by simpa using h))}
-    simp
+    simp only [self_getDual?_get_mem, true_and]
     rw [Finset.mapEmbedding_apply]
     simp
   exact Option.get_of_mem h h1
@@ -355,18 +375,18 @@ lemma insert_some_getDual?_neq_none (c : ContractionsNat n) (i : Fin n.succ) (j 
   apply Iff.intro
   · intro h
     have hk : (i.succAbove k) ∈ (insert c i (some j)).uncontracted := by
-      simp [uncontracted, -mem_uncontracted_insert_some_iff, ne_eq]
+      simp only [Nat.succ_eq_add_one, uncontracted, Finset.mem_filter, Finset.mem_univ, true_and]
       exact h
-    simp at hk
+    simp only [Nat.succ_eq_add_one, mem_uncontracted_insert_some_iff, ne_eq] at hk
     obtain ⟨z, hz1, hz2, hz3⟩ := hk
     rw [Function.Injective.eq_iff (Fin.succAbove_right_injective)] at hz1
     subst hz1
     simpa [uncontracted] using hz2
   · intro h
     have hk : (i.succAbove k) ∈ (insert c i (some j)).uncontracted := by
-      simp [mem_uncontracted_insert_some_iff]
+      simp only [Nat.succ_eq_add_one, mem_uncontracted_insert_some_iff, ne_eq]
       use k
-      simp [hkj]
+      simp only [hkj, not_false_eq_true, and_true, true_and]
       simpa [uncontracted] using h
     simpa [uncontracted, -mem_uncontracted_insert_some_iff, ne_eq] using hk
 
@@ -386,10 +406,11 @@ lemma insert_some_getDual?_neq_isSome_get (c : ContractionsNat n) (i : Fin n.suc
   have h1 : ((insert c i (some j)).getDual? (i.succAbove k))
     = some (i.succAbove ((c.getDual? k).get (by simpa [hkj] using h))) := by
     rw [getDual?_eq_some_iff_mem]
-    simp [insert]
+    simp only [Nat.succ_eq_add_one, insert, Finset.le_eq_subset, Finset.mem_insert, Finset.mem_map,
+      RelEmbedding.coe_toEmbedding]
     apply Or.inr
     use { k, ((c.getDual? k).get (by simpa [hkj] using h))}
-    simp
+    simp only [self_getDual?_get_mem, true_and]
     rw [Finset.mapEmbedding_apply]
     simp
   exact Option.get_of_mem h h1
@@ -409,9 +430,9 @@ lemma insert_some_getDual?_of_neq (c : ContractionsNat n) (i : Fin n.succ) (j : 
     have h2 :(c.getDual? k) = some ((c.getDual? k).get h) := by simp
     conv_rhs => rw [h2]
     rw [@Option.map_coe']
-  · simp at h
-    simp [h]
-    simp [hkj]
+  · simp only [Bool.not_eq_true, Option.not_isSome, Option.isNone_iff_eq_none] at h
+    simp only [Nat.succ_eq_add_one, h, Option.map_none']
+    simp only [ne_eq, hkj, not_false_eq_true, insert_some_getDual?_neq_none]
     exact h
 
 /-!
@@ -423,31 +444,32 @@ lemma insert_some_getDual?_of_neq (c : ContractionsNat n) (i : Fin n.succ) (j : 
 lemma insert_erase (c : ContractionsNat n) (i : Fin n.succ) (j : Option (c.uncontracted)) :
     erase (insert c i j) i = c := by
   refine Subtype.eq ?_
-  simp [insert, erase]
+  simp only [erase, Nat.succ_eq_add_one, insert, Finset.le_eq_subset]
   conv_rhs => rw [c.eq_filter_mem_self]
   refine Finset.filter_inj'.mpr ?_
   intro a _
   match j with
   | none =>
-    simp
+    simp only [Finset.mem_map, RelEmbedding.coe_toEmbedding]
     apply Iff.intro
     · intro ha
       obtain ⟨a', ha', ha''⟩ := ha
       rw [Finset.mapEmbedding_apply] at ha''
-      simp at ha''
+      simp only [Finset.map_inj] at ha''
       subst ha''
       exact ha'
     · intro ha
       use a
-      simp [ha]
+      simp only [ha, true_and]
       rw [Finset.mapEmbedding_apply]
   | some j =>
-    simp
+    simp only [Finset.mem_insert, Finset.mem_map, RelEmbedding.coe_toEmbedding]
     apply Iff.intro
     · intro ha
       rcases ha with ha | ha
       · have hin : ¬ i ∈ Finset.map i.succAboveEmb a := by
-          simp
+          simp only [Nat.succ_eq_add_one, Finset.mem_map, Fin.succAboveEmb_apply, not_exists,
+            not_and]
           intro x
           exact fun a => Fin.succAbove_ne i x
         refine False.elim (hin ?_)
@@ -455,13 +477,13 @@ lemma insert_erase (c : ContractionsNat n) (i : Fin n.succ) (j : Option (c.uncon
         simp
       · obtain ⟨a', ha', ha''⟩ := ha
         rw [Finset.mapEmbedding_apply] at ha''
-        simp at ha''
+        simp only [Finset.map_inj] at ha''
         subst ha''
         exact ha'
     · intro ha
       apply Or.inr
       use a
-      simp [ha]
+      simp only [ha, true_and]
       rw [Finset.mapEmbedding_apply]
 
 lemma insert_getDualErase (c : ContractionsNat n) (i : Fin n.succ) (j : Option c.uncontracted) :
@@ -469,7 +491,7 @@ lemma insert_getDualErase (c : ContractionsNat n) (i : Fin n.succ) (j : Option c
     uncontractedCongr (c := c) (c' := (c.insert i j).erase i) (by simp) j := by
   match n with
   | 0 =>
-    simp [getDualErase, insert]
+    simp only [insert, Nat.succ_eq_add_one, Nat.reduceAdd, Finset.le_eq_subset, getDualErase]
     fin_cases j
     simp
   | Nat.succ n =>
@@ -488,9 +510,9 @@ lemma erase_insert (c : ContractionsNat n.succ) (i : Fin n.succ) :
   match n with
   | 0 =>
     apply Subtype.eq
-    simp [getDualErase, insert]
+    simp only [Nat.succ_eq_add_one, Nat.reduceAdd, insert, getDualErase, Finset.le_eq_subset]
     ext a
-    simp
+    simp only [Finset.mem_map, RelEmbedding.coe_toEmbedding]
     apply Iff.intro
     · intro h
       simp only [erase, Nat.reduceAdd, Nat.succ_eq_add_one, Finset.mem_filter, Finset.mem_univ,
@@ -512,11 +534,12 @@ lemma erase_insert (c : ContractionsNat n.succ) (i : Fin n.succ) :
   apply Subtype.eq
   by_cases hi : (c.getDual? i).isSome
   · rw [insert_of_isSome]
-    simp [getDualErase, hi]
+    simp only [Nat.succ_eq_add_one, getDualErase, hi, ↓reduceDIte, Option.get_some,
+      Finset.le_eq_subset]
     rw [succsAbove_predAboveI]
     ext a
     apply Iff.intro
-    · simp
+    · simp only [Finset.mem_insert, Finset.mem_map, RelEmbedding.coe_toEmbedding]
       intro ha
       rcases ha with ha | ha
       · subst ha
@@ -525,26 +548,27 @@ lemma erase_insert (c : ContractionsNat n.succ) (i : Fin n.succ) :
         subst ha''
         simpa [erase] using ha'
     · intro ha
-      simp
+      simp only [Finset.mem_insert, Finset.mem_map, RelEmbedding.coe_toEmbedding]
       by_cases hia : a = {i, (c.getDual? i).get hi}
       · subst hia
         simp
       · apply Or.inr
-        simp [erase]
+        simp only [erase, Nat.succ_eq_add_one, Finset.mem_filter, Finset.mem_univ, true_and]
         obtain ⟨a', ha'⟩ := c.mem_not_eq_erase_of_isSome (a := a) i hi ha hia
         use a'
         simp_all only [Nat.succ_eq_add_one, true_and]
         obtain ⟨left, right⟩ := ha'
         subst right
         rfl
-    simp
+    simp only [Nat.succ_eq_add_one, ne_eq, self_neq_getDual?_get, not_false_eq_true]
     exact (getDualErase_isSome_iff_getDual?_isSome c i).mpr hi
-  · simp [getDualErase, hi, insert]
+  · simp only [Nat.succ_eq_add_one, insert, getDualErase, hi, Bool.false_eq_true, ↓reduceDIte,
+    Finset.le_eq_subset]
     ext a
-    simp
+    simp only [Finset.mem_map, RelEmbedding.coe_toEmbedding]
     apply Iff.intro
     · intro h
-      simp [erase] at h
+      simp only [erase, Nat.succ_eq_add_one, Finset.mem_filter, Finset.mem_univ, true_and] at h
       obtain ⟨a', ha', ha''⟩ := h
       subst ha''
       exact ha'
@@ -563,31 +587,32 @@ lemma erase_insert (c : ContractionsNat n.succ) (i : Fin n.succ) :
 /-- Lifts a contraction in `c` to a contraction in `(c.insert i j)`. -/
 def insertLift {c : ContractionsNat n} (i : Fin n.succ) (j : Option (c.uncontracted))
     (a : c.1) : (c.insert i j).1 := ⟨a.1.map (Fin.succAboveEmb i), by
-  simp [insert]
+  simp only [Nat.succ_eq_add_one, insert, Finset.le_eq_subset]
   match j with
   | none =>
-    simp
+    simp only [Finset.mem_map, RelEmbedding.coe_toEmbedding]
     use a
-    simp [a.2]
+    simp only [a.2, true_and]
     rfl
   | some j =>
-    simp
+    simp only [Finset.mem_insert, Finset.mem_map, RelEmbedding.coe_toEmbedding]
     apply Or.inr
     use a
-    simp [a.2]
+    simp only [a.2, true_and]
     rfl⟩
 
 lemma insertLift_injective {c : ContractionsNat n} (i : Fin n.succ) (j : Option (c.uncontracted)) :
     Function.Injective (insertLift i j) := by
   intro a b hab
-  simp [insertLift] at hab
+  simp only [Nat.succ_eq_add_one, insertLift, Subtype.mk.injEq, Finset.map_inj] at hab
   exact Subtype.eq hab
 
 lemma insertLift_none_surjective {c : ContractionsNat n} (i : Fin n.succ) :
     Function.Surjective (c.insertLift i none) := by
   intro a
   have ha := a.2
-  simp [Nat.succ_eq_add_one, insert, Finset.le_eq_subset,- Finset.coe_mem] at ha
+  simp only [Nat.succ_eq_add_one, insert, Finset.le_eq_subset, Finset.mem_map,
+    RelEmbedding.coe_toEmbedding] at ha
   obtain ⟨a', ha', ha''⟩ := ha
   use ⟨a', ha'⟩
   exact Subtype.eq ha''
@@ -602,10 +627,10 @@ lemma insert_fstFieldOfContract (c : ContractionsNat n) (i : Fin n.succ)
       i.succAbove (c.fstFieldOfContract a) := by
   refine (c.insert i j).eq_fstFieldOfContract_of_mem (a := (insertLift i j a))
     (i := i.succAbove (c.fstFieldOfContract a)) (j := i.succAbove (c.sndFieldOfContract a)) ?_ ?_ ?_
-  · simp [insertLift]
+  · simp only [Nat.succ_eq_add_one, insertLift, Finset.mem_map, Fin.succAboveEmb_apply]
     use (c.fstFieldOfContract a)
     simp
-  · simp [insertLift]
+  · simp only [Nat.succ_eq_add_one, insertLift, Finset.mem_map, Fin.succAboveEmb_apply]
     use (c.sndFieldOfContract a)
     simp
   · refine Fin.succAbove_lt_succAbove_iff.mpr ?_
@@ -617,10 +642,10 @@ lemma insert_sndFieldOfContract (c : ContractionsNat n) (i : Fin n.succ)
     i.succAbove (c.sndFieldOfContract a) := by
   refine (c.insert i j).eq_sndFieldOfContract_of_mem (a := (insertLift i j a))
     (i := i.succAbove (c.fstFieldOfContract a)) (j := i.succAbove (c.sndFieldOfContract a)) ?_ ?_ ?_
-  · simp [insertLift]
+  · simp only [Nat.succ_eq_add_one, insertLift, Finset.mem_map, Fin.succAboveEmb_apply]
     use (c.fstFieldOfContract a)
     simp
-  · simp [insertLift]
+  · simp only [Nat.succ_eq_add_one, insertLift, Finset.mem_map, Fin.succAboveEmb_apply]
     use (c.sndFieldOfContract a)
     simp
   · refine Fin.succAbove_lt_succAbove_iff.mpr ?_
@@ -658,25 +683,26 @@ lemma insertLiftSome_injective {c : ContractionsNat n} (i : Fin n.succ) (j : c.u
         i.succAbove (c.sndFieldOfContract a)} : Finset (Fin (n + 1))) := by
       rw [hab]
       simp
-    simp at hi
+    simp only [Nat.succ_eq_add_one, Finset.mem_insert, Finset.mem_singleton] at hi
     rcases hi with hi | hi
     · exact False.elim (Fin.ne_succAbove _ _ hi)
     · exact False.elim (Fin.ne_succAbove _ _ hi)
   | Sum.inr a, Sum.inr b =>
-    simp [insertLiftSome] at hab
+    simp only [Nat.succ_eq_add_one, insertLiftSome] at hab
     simpa using insertLift_injective i (some j) hab
 
 lemma insertLiftSome_surjective {c : ContractionsNat n} (i : Fin n.succ) (j : c.uncontracted) :
     Function.Surjective (insertLiftSome i j) := by
   intro a
   have ha := a.2
-  simp [Nat.succ_eq_add_one, insert, Finset.le_eq_subset, - Finset.coe_mem] at ha
+  simp only [Nat.succ_eq_add_one, insert, Finset.le_eq_subset, Finset.mem_insert, Finset.mem_map,
+    RelEmbedding.coe_toEmbedding] at ha
   rcases ha with ha | ha
   · use Sum.inl ()
     exact Subtype.eq ha.symm
   · obtain ⟨a', ha', ha''⟩ := ha
     use Sum.inr ⟨a', ha'⟩
-    simp [insertLiftSome, insertLift]
+    simp only [Nat.succ_eq_add_one, insertLiftSome, insertLift]
     exact Subtype.eq ha''
 
 lemma insertLiftSome_bijective {c : ContractionsNat n} (i : Fin n.succ) (j : c.uncontracted) :
